Ground typing for prob terms + env changes and var containment

theories/ProbTerms.v
@@ -1,7 +1,7 @@
 (* ProbTerms.v *)
 (* Probabilistic terms *)
 From EasyUCFormalization Require Import NonProbTerms.
-From Coq Require Import QArith.
+Require Import QArith String.
 
 (* Distribution type *)
 Inductive dty : Type :=
@@ -16,19 +16,54 @@ Inductive dtm : Type :=
   (* Product terms *)
   | DTm_Prod : list dtm -> dtm.
 
+(* Ground typing for distribution terms *)
+Inductive dtm_has_ground_type (env : env) : dtm -> ty -> Prop :=
+  | DtmUniformHasTy_Int : forall (t1 t2 : tm),
+    tm_has_type env t1 Ty_Int ->
+    tm_has_type env t2 Ty_Int ->
+    dtm_has_ground_type env (DTm_Uniform t1 t2) Ty_Int
+  | DtmCastHasTy : forall (t : tm) (ty : ty),
+    tm_has_type env t ty ->
+    dtm_has_ground_type env (DTm_Cast t) ty
+  | DtmEmptyProdHasTy :
+    dtm_has_ground_type env (DTm_Prod nil) (Ty_Prod nil)
+  | DtmNEProdHasTy : forall (htm : dtm) (ltm : list dtm) (hty : ty) (lty : list ty),
+    dtm_has_ground_type env htm hty ->
+    dtm_has_ground_type env (DTm_Prod ltm) (Ty_Prod lty) ->
+    dtm_has_ground_type env (DTm_Prod (htm :: ltm)) (Ty_Prod (hty :: lty)).
+
 (* Semantics for distribution terms *)
 (* Relation on distribution terms and pairs of values and probabilities *)
-Inductive deval : dtm -> (val * Q) -> Prop :=
+Inductive deval (env : env) : dtm -> (val * Q) -> Prop :=
   | DEval_Uniform : forall (t1 t2 : tm) (n1 n2 elt : Z),
-    eval t1 (Val_Int n1) -> 
-    eval t2 (Val_Int n2) -> 
+    eval env t1 (Val_Int n1) -> 
+    eval env t2 (Val_Int n2) -> 
     (n1 <= elt <= n2)%Z ->
-    deval (DTm_Uniform t1 t2) (Val_Int elt, 1 # (Z.to_pos (n2 - n1 + 1)))
+    deval env (DTm_Uniform t1 t2) (Val_Int elt, 1 # (Z.to_pos (n2 - n1 + 1)))
   | DEval_Cast : forall (t : tm) (v : val),
-    eval t v ->
-    deval (DTm_Cast t) (v, 1)
+    eval env t v ->
+    deval env (DTm_Cast t) (v, 1)
   | DEval_Prod : forall (ht : dtm) (hv : val) 
       (lt : list dtm) (lv : list val) (hprob lprob : Q),
-    deval ht (hv, hprob) ->
-    deval (DTm_Prod lt) (Val_Prod lv, lprob) ->
-    deval (DTm_Prod (ht :: lt)) (Val_Prod (hv :: lv), hprob * lprob).
+    deval env ht (hv, hprob) ->
+    deval env (DTm_Prod lt) (Val_Prod lv, lprob) ->
+    deval env (DTm_Prod (ht :: lt)) (Val_Prod (hv :: lv), hprob * lprob).
+
+Theorem deterministic_eval_to_probabilistic_eval : forall (env : env) (t : tm) (v : val),
+  eval env t v -> deval env (DTm_Cast t) (v, 1).
+Proof.
+  intros t v H.
+  apply DEval_Cast.
+Qed.
+
+(* Check whether a distribution term contains a variable *)
+Inductive dtm_contains_var : dtm -> string -> Prop :=
+  | DtmContainsVar_Uniform : forall (t1 t2 : tm) (x : string),
+    (tm_contains_var t1 x \/ tm_contains_var t2 x) -> 
+    dtm_contains_var (DTm_Uniform t1 t2) x
+  | DtmContainsVar_Cast : forall (t : tm) (x : string),
+    tm_contains_var t x -> 
+    dtm_contains_var (DTm_Cast t) x
+  | DtmContainsVar_Prod : forall (htm : dtm) (ltm : list dtm) (x : string),
+    (dtm_contains_var htm x \/ dtm_contains_var (DTm_Prod ltm) x) ->
+    dtm_contains_var (DTm_Prod (htm :: ltm)) x.
